changes

NewTranslate/No_Translate.thy
@@ -3,41 +3,104 @@ theory No_Translate
     "Main"
     "../General/Relations"
     "HOL-Hoare_Parallel.Quote_Antiquote"
-
+    "HOL-Examples.Records"
+    "../Programming/State_Relations"
+    "../Programming/Specification"
+    "../General/Sequential"
 begin
 
 text \<open>We use (\<lpred>p\<rpred>) to give a relation where (\<sigma>,\<sigma>') satisfy predicate p\<close>
-
+(*
 syntax
   "_rel" :: "(('a*'a) \<Rightarrow> bool) \<Rightarrow> 'a rel" ("\<lpred>_\<rpred>" [0] 1000)
   "_set" :: "('a \<Rightarrow> bool) \<Rightarrow> 'a set" ("\<lrel>_\<rrel>" [0] 1000)
   "_comp" :: "[('b * 'c) set, ('a * 'b) set] \<Rightarrow> ('a * 'c) set" (infixr "\<Zsemi>" 75)
-  "_dunno" :: "'a rel \<Rightarrow> 'a set \<Rightarrow> 'a set" ("_\<lparr>_\<rparr>" [0] 1000)
 
 translations
   "\<lpred> r \<rpred>" \<rightharpoonup> "CONST Collect(_quote r)"
   "\<lrel> p \<rrel>" \<rightharpoonup> "CONST Collect(_quote p)"
   "r \<Zsemi> s" \<rightharpoonup> "r O s"
-  "r\<lparr>p\<rparr>" \<rightharpoonup> "{s'. \<exists>s\<in>p. (s, s')\<in>r}"
+*)
+definition relation :: "(('a*'a) \<Rightarrow> bool) \<Rightarrow> 'a rel" ("\<lpred>_\<rpred>" [30])
+  where "relation r \<equiv> {(s, s') \<in> UNIV. r (s, s')} "
 
-lemma strengthen_pre: "(\<lpred>p1\<rpred> \<subseteq> \<lpred>p2\<rpred>) \<equiv> p1 \<Longrightarrow> p2"
-  by blast
+definition predset :: "('a \<Rightarrow> bool) \<Rightarrow> 'a set" ("\<lrel>_\<rrel>" [30])
+  where "predset p = Collect(p)"
 
-lemma dom_restrict: "(\<lrel>p\<rrel> \<triangleleft> \<lpred>q2\<rpred> \<subseteq> \<lpred>q1\<rpred>) \<equiv> p \<and> q2 \<Longrightarrow> q1"
-  by (smt (verit, del_insts) IntE IntI case_prodE case_prodI2 mem_Collect_eq restrict_domain_def subsetI subset_empty)
+(* Set containing \<dots>*)
+definition dunno :: "('a*'a \<Rightarrow> bool) \<Rightarrow> ('a \<Rightarrow> bool) \<Rightarrow> 'a set" ("_\<bar>_\<bar>" [30,30])
+  where "dunno r p \<equiv> {s'. (\<exists> s. p s \<and> r (s,s'))}"
 
-lemma range_restrict: "(\<lpred>q2\<rpred> \<triangleright> \<lrel>p\<rrel> \<subseteq> \<lpred>q1\<rpred>) \<equiv> p \<and> q2 \<Longrightarrow> q1"
-  by (smt (verit, ccfv_threshold) Collect_empty_eq IntI case_prodE case_prodI inf_le2 mem_Collect_eq range_restrict_remove restrict_range_def subsetD)
+lemma strengthen_pre: "(\<lrel>p1\<rrel> \<subseteq> \<lrel>p2\<rrel>) \<Longrightarrow> (\<And>s. p1 s \<Longrightarrow> p2 s)"
+  by (simp add: Collect_mono_iff predset_def)
+
+lemma dom_restrict: "(\<lrel>p\<rrel> \<triangleleft> \<lpred>q2\<rpred> \<subseteq> \<lpred>q1\<rpred>) \<Longrightarrow> (\<And>s. p (fst s) \<and> q2 s \<Longrightarrow> q1 s)"
+  by (smt (verit) Int_def UNIV_def in_mono mem_Collect_eq predset_def prod.collapse relation_def restrict_domain_def split_conv)
+
+lemma range_restrict: "(\<lpred>q2\<rpred> \<triangleright> \<lrel>p\<rrel> \<subseteq> \<lpred>q1\<rpred>) \<Longrightarrow> (\<And>s. p (snd s) \<and> q2 s \<Longrightarrow> q1 s)"
+  by (smt (verit, del_insts) IntI in_mono mem_Collect_eq predset_def prod.collapse relation_def restrict_range_def split_def top_greatest)
+
+lemma "(Range (\<lrel>p\<rrel> \<triangleleft> \<lpred>r\<rpred>)) \<subseteq> (r\<bar>p\<bar>)"
+  by (smt (verit, best) IntE RangeE dunno_def mem_Collect_eq predset_def relation_def restrict_domain_def split_conv subsetI)
+
+lemma "(r\<bar>p\<bar>) \<subseteq> (Range (\<lrel>p\<rrel> \<triangleleft> \<lpred>r\<rpred>))"
+  by (smt (verit, ccfv_threshold) Int_iff Int_iff Range.intros Range.intros Range_mono UNIV_def case_prodE case_prod_conv case_prod_unfold domain_restrict_remove dunno_def in_mono inf.orderE mem_Collect_eq mem_Collect_eq mem_Collect_eq predset_def prod.collapse prod.collapse prod.inject prod.inject relation_def restrict_domain_def subsetD subsetI)
 
 
 
-
-
-
-record vars =
+record 'a vars =
   x :: nat
+  \<dots> :: 'a
 
-lemma id_rel: "\<lpred>s x = s' x\<rpred> \<equiv> (Id :: vars rel)"
-  sorry
+(*
+definition id_rel :: "('a*'a) \<Rightarrow> bool" where
+"id_rel s \<equiv> (fst s = snd s)"
 
+lemma "Id = \<lpred>id_rel\<rpred>"
+  by (metis (mono_tags, lifting) Collect_cong Id_fstsnd_eq UNIV_I id_rel_def prod.collapse relation_def split_def)
+*)
+
+(*
+function id_rel_param :: "'b list \<Rightarrow> ('a vars * 'a vars) \<Rightarrow> bool" where
+"id_rel_param (p#ps) s = id_rel_param ps ( s\<lparr>p := ( p (fst s) )\<rparr> ) " | 
+"id_rel_param [] s = id_rel s"
+*)
+
+context state_relations
+begin
+definition id_rel :: "('state*'state) \<Rightarrow> bool" where
+"id_rel s \<equiv> \<forall>x. ((get_var x (fst s)) = (get_var x (snd s)))"
+
+definition id_rel_bar :: "'varname fset \<Rightarrow> ('state*'state) \<Rightarrow> bool" where
+"id_rel_bar xs s \<equiv> \<forall>x :: 'varname. x|\<notin>|xs \<longrightarrow> ((get_var x (fst s)) = (get_var x (snd s)))"
+
+lemma "\<lpred>id_rel\<rpred> \<subseteq> id_bar xs"
+  by (smt (verit, ccfv_SIG) fst_conv id_rel_def mem_Collect_eq relation_def snd_conv split_conv state_relations.id_bar_def state_relations_axioms subrelI)
+
+lemma "\<lpred>id_rel\<rpred> = id_bar fempty"
+  by (smt (verit, ccfv_SIG) Collect_cong UNIV_I ex_fin_conv id_bar_def id_rel_def prod.collapse relation_def split_def)
+
+lemma "\<lpred>id_rel_bar xs\<rpred> = id_bar xs"
+  by (smt (verit, del_insts) Collect_cong UNIV_I case_prod_unfold fst_conv id_bar_def id_rel_bar_def relation_def snd_conv)
+end
+
+locale ctxt = strong_spec + seq 
+
+text \<open>Below are some results around program refinement\<close>
+context strong_spec
+begin
+lemma 
+  assumes "\<And>x. p1 x \<Longrightarrow> p2 x"
+  shows "\<lbrace>\<lrel>p1\<rrel>\<rbrace> \<ge> \<lbrace>\<lrel>p2\<rrel>\<rbrace>"
+  by (metis Collect_mono assert_iso assms predset_def)
+
+lemma 
+  assumes "\<And>s s'. (p s \<and> q2 (s, s')) \<Longrightarrow> q1 (s, s')"
+  shows "\<lbrace>\<lrel>p\<rrel>\<rbrace>;\<lparr>\<lpred>q1\<rpred>\<rparr> \<ge> \<lbrace>\<lrel>p\<rrel>\<rbrace>;\<lparr>\<lpred>q2\<rpred>\<rparr>"
+proof - 
+  have "\<And>s s'. (p s \<and> q2 (s, s')) \<Longrightarrow> (p \<triangleleft> q1)" by sledgehammer
+
+
+
+end
 end
